Add addBefore working

project.dfy
@@ -32,11 +32,11 @@ module Collections {
 
         ghost var omDsSeq: seq<int>;
 
-        // NOTE: Trait level invariants are not working
+        // NOTE: Trait level invariants are not working. Invalid Class/Trait member in Dafny grammar
         // invariant forall fstSeq, scndSeq, val :: omDsSeq == fstSeq + [val] + scndSeq && val !in fstSeq + scndSeq;
 
         // Check all the values are unique
-        predicate checkUnique()
+        ghost predicate checkUnique()
         {
             forall fstSeq, scndSeq, val :: omDsSeq == fstSeq + [val] + scndSeq && val !in fstSeq + scndSeq
         }
@@ -51,73 +51,73 @@ module Collections {
             // Check x's position is less than y's position
             ensures exists fstSeq, scndSeq :: old(omDsSeq) == fstSeq + [yNode.omValue] + scndSeq && omDsSeq == fstSeq + [x, yNode.omValue] + scndSeq
 
-        method addAfter(x: int, yNode: Node)
-            // Check y exists in DS
-            requires yNode.omValue in omDsSeq
-            // Check x doesn't exist in DS
-            requires x !in omDsSeq
-            // Check all the values are unique
-            requires checkUnique()
-            // Check x's position is greater than y's position
-            ensures exists fstSeq, scndSeq :: old(omDsSeq) == fstSeq + [yNode.omValue] + scndSeq && omDsSeq == fstSeq + [yNode.omValue, x] + scndSeq
+        // method addAfter(x: int, yNode: Node)
+        //     // Check y exists in DS
+        //     requires yNode.omValue in omDsSeq
+        //     // Check x doesn't exist in DS
+        //     requires x !in omDsSeq
+        //     // Check all the values are unique
+        //     requires checkUnique()
+        //     // Check x's position is greater than y's position
+        //     ensures exists fstSeq, scndSeq :: old(omDsSeq) == fstSeq + [yNode.omValue] + scndSeq && omDsSeq == fstSeq + [yNode.omValue, x] + scndSeq
 
-        // Inserts x at the start of the linked list
-        method add(x: int)
-            // Check x doesn't exist in DS
-            requires x !in omDsSeq
-            // Check all the values are unique
-            requires checkUnique()
-            // Check x exists random position in DS
-            ensures x in omDsSeq
+        // // Inserts x at the start of the linked list
+        // method add(x: int)
+        //     // Check x doesn't exist in DS
+        //     requires x !in omDsSeq
+        //     // Check all the values are unique
+        //     requires checkUnique()
+        //     // Check x exists random position in DS
+        //     ensures x in omDsSeq
 
-        method element(x: int) returns (exist: bool)
-            // At some position, if x exists then return true otherwise false
-            ensures exist == (x in omDsSeq)
+        // method element(x: int) returns (exist: bool)
+        //     // At some position, if x exists then return true otherwise false
+        //     ensures exist == (x in omDsSeq)
 
-        method before(xNode: Node, yNode: Node) returns (isBefore: bool)
-            // Checks x and y are different values
-            requires xNode.omValue != yNode.omValue
-            // Check x exists in DS
-            requires xNode.omValue in omDsSeq
-            // Check y exists in DS
-            requires yNode.omValue in omDsSeq
-            // Check all the values are unique
-            requires checkUnique()
-            // If x's position is less than y's position then return true otherwise false
-            ensures exists fstSeq, scndSeq :: omDsSeq == fstSeq + [xNode.omValue] + scndSeq && isBefore == (yNode.omValue in scndSeq)
+        // method before(xNode: Node, yNode: Node) returns (isBefore: bool)
+        //     // Checks x and y are different values
+        //     requires xNode.omValue != yNode.omValue
+        //     // Check x exists in DS
+        //     requires xNode.omValue in omDsSeq
+        //     // Check y exists in DS
+        //     requires yNode.omValue in omDsSeq
+        //     // Check all the values are unique
+        //     requires checkUnique()
+        //     // If x's position is less than y's position then return true otherwise false
+        //     ensures exists fstSeq, scndSeq :: omDsSeq == fstSeq + [xNode.omValue] + scndSeq && isBefore == (yNode.omValue in scndSeq)
 
-        method append(x: int)
-            // Check x doesn't exist in DS
-            requires x !in omDsSeq
-            // Check all the values are unique
-            requires checkUnique()
-            // Check val is at the end of the DS always.
-            ensures omDsSeq == old(omDsSeq) + x
-            // Check all the values are unique. This is an additional check
-            ensures checkUnique()
+        // method append(x: int)
+        //     // Check x doesn't exist in DS
+        //     requires x !in omDsSeq
+        //     // Check all the values are unique
+        //     requires checkUnique()
+        //     // Check val is at the end of the DS always.
+        //     ensures omDsSeq == old(omDsSeq) + x
+        //     // Check all the values are unique. This is an additional check
+        //     ensures checkUnique()
 
-        method prepend(x: int)
-            // Check x doesn't exist in DS
-            requires x !in omDsSeq
-            // Check all the values are unique
-            requires checkUnique()
-            // Check x is at the start of the DS always
-            ensures omDsSeq == x + old(omDsSeq)
-            // Check all the values are unique. This is an additional check
-            ensures checkUnique()
+        // method prepend(x: int)
+        //     // Check x doesn't exist in DS
+        //     requires x !in omDsSeq
+        //     // Check all the values are unique
+        //     requires checkUnique()
+        //     // Check x is at the start of the DS always
+        //     ensures omDsSeq == x + old(omDsSeq)
+        //     // Check all the values are unique. This is an additional check
+        //     ensures checkUnique()
 
-        method remove(xNode: Node)
-            // Check x exists in DS
-            requires xNode.omValue in omDsSeq
-            // Check all the values are unique
-            requires checkUnique()
-            // Check x doesn't exist in DS
-            ensures xNode.omValue !in omDsSeq
+        // method remove(xNode: Node)
+        //     // Check x exists in DS
+        //     requires xNode.omValue in omDsSeq
+        //     // Check all the values are unique
+        //     requires checkUnique()
+        //     // Check x doesn't exist in DS
+        //     ensures xNode.omValue !in omDsSeq
 
-        method getXNode(x: int) returns (node: Node)
-            // Check x exists in DS
-            requires x in omDsSeq
-            ensures node.omValue == x
+        // method getXNode(x: int) returns (node: Node)
+        //     // Check x exists in DS
+        //     requires x in omDsSeq
+        //     ensures node.omValue == x
     }
 
     class OMDataStruct extends OMDataStructTrait {
@@ -140,15 +140,15 @@ module Collections {
         function getLength(): int
         {
             // Just to work aorund previous is Node? nullable
-            if taildNode.previous == null then 0 else
-            if taildNode.previous == headNode then 0 else taildNode.previous.index + 1
+            if tail.previous == null then 0 else
+            if tail.previous == head then 0 else tail.previous.index + 1
         }
 
         // To be used in decrease clause
         function getCurrentLength(node: Node?): int
         {
             if node.next == null then 0 else
-            if node.next == tailNode then 0 else 1 + getCurrentLength(node.next)
+            if node.next == tail then 0 else 1 + getCurrentLength(node.next)
         }
 
         method addBefore(x: int, yNode: Node)
@@ -156,16 +156,14 @@ module Collections {
             requires yNode.omValue in omDsSeq
             // Check x doesn't exist in DS
             requires x !in omDsSeq
-            requires oldOmDsSeq == omDsSeq
-            // Check each value is unique
-            requires exists fstSeq, scndSeq, val :: omDsSeq == fstSeq + [val] + scndSeq && val !in fstSeq + scndSeq
+            // Check all the values are unique
+            requires checkUnique()
             // Check x's position is less than y's position
-            ensures exists fstSeq, scndSeq :: oldOmDsSeq == fstSeq + [yNode.omValue] + scndSeq && omDsSeq == fstSeq + [x, yNode.omValue] + scndSeq
+            ensures exists fstSeq, scndSeq :: old(omDsSeq) == fstSeq + [yNode.omValue] + scndSeq && omDsSeq == fstSeq + [x, yNode.omValue] + scndSeq
             modifies yNode, yNode.previous
         {
             // yNode.previous always not null since it can be head node in the worst case.
             if(yNode.previous != null) {
-                assert oldOmDsSeq == omDsSeq;
 
                 var labelGap: int := yNode.omLabel - yNode.previous.omLabel;
                 var xLabel: int := yNode.previous.omLabel + (labelGap / 2);
@@ -185,234 +183,234 @@ module Collections {
             reIndex();
         }
 
-        method addAfter(x: int, yNode: Node)
-            // Check y exists in DS
-            requires yNode.omValue in omDsSeq
-            // Check x doesn't exist in DS
-            requires x !in omDsSeq
-            requires oldOmDsSeq == omDsSeq
-            // Check each value is unique
-            requires exists fstSeq, scndSeq, val :: omDsSeq == fstSeq + [val] + scndSeq && val !in fstSeq + scndSeq
-            // Check x's position is greater than y's position
-            ensures exists fstSeq, scndSeq :: oldOmDsSeq == fstSeq + [yNode.omValue] + scndSeq && omDsSeq == fstSeq + [x, yNode.omValue] + scndSeq
-            modifies yNode, yNode.next
-        {
-            // yNode.next always not null since it can be tail node in the worst case.
-            if(yNode.next != null) {
-                assert oldOmDsSeq == omDsSeq;
-
-                var labelGap: int := yNode.omLabel - yNode.next.omLabel;
-                var xLabel: int := yNode.next.omLabel + (labelGap / 2);
-                var xNode: Node := new Node(xLabel, x, yNode.index+1);
-
-                var nextNode: Node := yNode.next;
-                xNode.previous := yNode;
-                xNode.next := nextNode;
-                nextNode.previous := xNode;
-                yNode.next := xNode;
-            }
-
-            omDsSeq := omDsSeq[..yNode.index+1] + [x] + omDsSeq[yNode.index+1..];
-            assert tail.previous.index+1 == |omDsSeq|;
-            assert omDsSeq[yNode.index+1] == x;
-
-            reIndex();
-        }
-
-        // Inserts x at the start of the linked list
-        method add(x: int)
-            // Check x doesn't exist in DS
-            requires x !in omDsSeq
-            // Check each value is unique
-            requires exists fstSeq, scndSeq, val :: omDsSeq == fstSeq + [val] + scndSeq && val !in fstSeq + scndSeq
-            // Check x exists random position in DS
-            ensures x in omDsSeq
-            modifies head, head.next
-        {
-            // head.next always not null since it can be tail node in the worst case.
-            if(head.next != null) {
-
-                var nextNode: Node := head.next;
-
-                var labelGap: int := nextNode.omLabel - head.omLabel;
-                var xLabel: int := head.omLabel + (labelGap / 2);
-                var xNode: Node := new Node(xLabel, x, 0);
-
-                xNode.previous := head;
-                xNode.next := nextNode;
-                nextNode.previous := xNode;
-                head.next := xNode;
-            }
-
-            omDsSeq := [x] + omDsSeq[..];
-            assert tail.previous.index+1 == |omDsSeq|;
-            assert omDsSeq[0] == x;
-            
-            reIndex();
-        }
-
-        method element(x: int) returns (exist: bool)
-            // At some position, if x exists then return true otherwise false
-            ensures exist == (x in omDsSeq)
-        {
-            exist := false;
-            var iNode: Node? := head.next;
-            while(iNode != null && iNode != tail)
-                invariant iNode == null || (iNode == tail || iNode != tail)
-                decreases iNode
-            {
-                if(iNode.omValue == x) {
-                    exist := true;
-                    break;
-                }
-
-                iNode := iNode.next;
-            }
-
-            assert (x in omDsSeq) && exist;
-        }
-
-        method before(xNode: Node, yNode: Node) returns (isBefore: bool)
-            // Checks x and y are different values
-            requires xNode.omValue != yNode.omValue
-            // Check x exists in DS
-            requires xNode.omValue in omDsSeq
-            // Check y exists in DS
-            requires yNode.omValue in omDsSeq
-            // Check each value is unique
-            requires exists fstSeq, scndSeq, val :: omDsSeq == fstSeq + [val] + scndSeq && val !in fstSeq + scndSeq
-            // If x's position is less than y's position then return true otherwise false
-            ensures exists fstSeq, midSeq, scndSeq :: omDsSeq == fstSeq + [xNode.omValue] + midSeq + [yNode.omValue] + scndSeq
-        {
-            if(xNode.omLabel < yNode.omLabel) {
-                isBefore := true;
-            } else {
-                isBefore := false;
-            }
-            
-            // ghost var xIndex: int := findXIndex(xNode.omValue, head.next);
-            // ghost var yIndex: int := findXIndex(yNode.omValue, head.next);
-            // assert xIndex < yIndex;
-        }
-
-        // function findXIndex(x: int, node: Node?): int
-        //     decreases node == null || node.next == tail
+        // method addAfter(x: int, yNode: Node)
+        //     // Check y exists in DS
+        //     requires yNode.omValue in omDsSeq
+        //     // Check x doesn't exist in DS
+        //     requires x !in omDsSeq
+        //     requires oldOmDsSeq == omDsSeq
+        //     // Check each value is unique
+        //     requires exists fstSeq, scndSeq, val :: omDsSeq == fstSeq + [val] + scndSeq && val !in fstSeq + scndSeq
+        //     // Check x's position is greater than y's position
+        //     ensures exists fstSeq, scndSeq :: oldOmDsSeq == fstSeq + [yNode.omValue] + scndSeq && omDsSeq == fstSeq + [x, yNode.omValue] + scndSeq
+        //     modifies yNode, yNode.next
         // {
-        //     if node == null then -1 else
-        //     if node == tail then -1 else
-        //     if node.omValue == x then node.index else findXIndex(x, node.next)
+        //     // yNode.next always not null since it can be tail node in the worst case.
+        //     if(yNode.next != null) {
+        //         assert oldOmDsSeq == omDsSeq;
+
+        //         var labelGap: int := yNode.omLabel - yNode.next.omLabel;
+        //         var xLabel: int := yNode.next.omLabel + (labelGap / 2);
+        //         var xNode: Node := new Node(xLabel, x, yNode.index+1);
+
+        //         var nextNode: Node := yNode.next;
+        //         xNode.previous := yNode;
+        //         xNode.next := nextNode;
+        //         nextNode.previous := xNode;
+        //         yNode.next := xNode;
+        //     }
+
+        //     omDsSeq := omDsSeq[..yNode.index+1] + [x] + omDsSeq[yNode.index+1..];
+        //     assert tail.previous.index+1 == |omDsSeq|;
+        //     assert omDsSeq[yNode.index+1] == x;
+
+        //     reIndex();
         // }
 
-        method append(valSet: set<int>)
-            // Check x doesn't exist in DS
-            requires exists val :: val in valSet && val !in omDsSeq
-            requires oldOmDsSeq == omDsSeq
-            // Check each value is unique
-            requires exists fstSeq, scndSeq, val :: omDsSeq == fstSeq + [val] + scndSeq && val !in fstSeq + scndSeq
-            // If DS size is 1 then x is at the start of DS or DS size is greater than 1 then x is at the end of the DS.
-            ensures exists fstSeq, scndSeq, val :: omDsSeq == fstSeq + scndSeq && oldOmDsSeq == fstSeq && val in scndSeq && val in valSet
-            // Check each value is unique
-            ensures exists fstSeq, scndSeq, val :: omDsSeq == fstSeq + [val] + scndSeq && val !in fstSeq + scndSeq
-        {
-            var iValSet := valSet;
-            while ( iValSet != {} )
-                decreases iValSet;
-                modifies tail.previous
-            {
-                var setVal :| setVal in iValSet;
+        // // Inserts x at the start of the linked list
+        // method add(x: int)
+        //     // Check x doesn't exist in DS
+        //     requires x !in omDsSeq
+        //     // Check each value is unique
+        //     requires exists fstSeq, scndSeq, val :: omDsSeq == fstSeq + [val] + scndSeq && val !in fstSeq + scndSeq
+        //     // Check x exists random position in DS
+        //     ensures x in omDsSeq
+        //     modifies head, head.next
+        // {
+        //     // head.next always not null since it can be tail node in the worst case.
+        //     if(head.next != null) {
+
+        //         var nextNode: Node := head.next;
+
+        //         var labelGap: int := nextNode.omLabel - head.omLabel;
+        //         var xLabel: int := head.omLabel + (labelGap / 2);
+        //         var xNode: Node := new Node(xLabel, x, 0);
+
+        //         xNode.previous := head;
+        //         xNode.next := nextNode;
+        //         nextNode.previous := xNode;
+        //         head.next := xNode;
+        //     }
+
+        //     omDsSeq := [x] + omDsSeq[..];
+        //     assert tail.previous.index+1 == |omDsSeq|;
+        //     assert omDsSeq[0] == x;
+            
+        //     reIndex();
+        // }
+
+        // method element(x: int) returns (exist: bool)
+        //     // At some position, if x exists then return true otherwise false
+        //     ensures exist == (x in omDsSeq)
+        // {
+        //     exist := false;
+        //     var iNode: Node? := head.next;
+        //     while(iNode != null && iNode != tail)
+        //         invariant iNode == null || (iNode == tail || iNode != tail)
+        //         decreases iNode
+        //     {
+        //         if(iNode.omValue == x) {
+        //             exist := true;
+        //             break;
+        //         }
+
+        //         iNode := iNode.next;
+        //     }
+
+        //     assert (x in omDsSeq) && exist;
+        // }
+
+        // method before(xNode: Node, yNode: Node) returns (isBefore: bool)
+        //     // Checks x and y are different values
+        //     requires xNode.omValue != yNode.omValue
+        //     // Check x exists in DS
+        //     requires xNode.omValue in omDsSeq
+        //     // Check y exists in DS
+        //     requires yNode.omValue in omDsSeq
+        //     // Check each value is unique
+        //     requires exists fstSeq, scndSeq, val :: omDsSeq == fstSeq + [val] + scndSeq && val !in fstSeq + scndSeq
+        //     // If x's position is less than y's position then return true otherwise false
+        //     ensures exists fstSeq, midSeq, scndSeq :: omDsSeq == fstSeq + [xNode.omValue] + midSeq + [yNode.omValue] + scndSeq
+        // {
+        //     if(xNode.omLabel < yNode.omLabel) {
+        //         isBefore := true;
+        //     } else {
+        //         isBefore := false;
+        //     }
+            
+        //     // ghost var xIndex: int := findXIndex(xNode.omValue, head.next);
+        //     // ghost var yIndex: int := findXIndex(yNode.omValue, head.next);
+        //     // assert xIndex < yIndex;
+        // }
+
+        // // function findXIndex(x: int, node: Node?): int
+        // //     decreases node == null || node.next == tail
+        // // {
+        // //     if node == null then -1 else
+        // //     if node == tail then -1 else
+        // //     if node.omValue == x then node.index else findXIndex(x, node.next)
+        // // }
+
+        // method append(valSet: set<int>)
+        //     // Check x doesn't exist in DS
+        //     requires exists val :: val in valSet && val !in omDsSeq
+        //     requires oldOmDsSeq == omDsSeq
+        //     // Check each value is unique
+        //     requires exists fstSeq, scndSeq, val :: omDsSeq == fstSeq + [val] + scndSeq && val !in fstSeq + scndSeq
+        //     // If DS size is 1 then x is at the start of DS or DS size is greater than 1 then x is at the end of the DS.
+        //     ensures exists fstSeq, scndSeq, val :: omDsSeq == fstSeq + scndSeq && oldOmDsSeq == fstSeq && val in scndSeq && val in valSet
+        //     // Check each value is unique
+        //     ensures exists fstSeq, scndSeq, val :: omDsSeq == fstSeq + [val] + scndSeq && val !in fstSeq + scndSeq
+        // {
+        //     var iValSet := valSet;
+        //     while ( iValSet != {} )
+        //         decreases iValSet;
+        //         modifies tail.previous
+        //     {
+        //         var setVal :| setVal in iValSet;
                 
-                // tail.previous is head node in the worst case and never be null
-                // check whether existing element or not otherwise ignore to keep the uniqueness
-                var existSetVal: bool := element(setVal);
-                if(tail.previous != null && !existSetVal) {
-                    var prevNode: Node := tail.previous;
-                    var labelGap: int := tail.omLabel - prevNode.omLabel;
+        //         // tail.previous is head node in the worst case and never be null
+        //         // check whether existing element or not otherwise ignore to keep the uniqueness
+        //         var existSetVal: bool := element(setVal);
+        //         if(tail.previous != null && !existSetVal) {
+        //             var prevNode: Node := tail.previous;
+        //             var labelGap: int := tail.omLabel - prevNode.omLabel;
 
-                    if(labelGap == 0) {
-                        relabel();
-                    }
+        //             if(labelGap == 0) {
+        //                 relabel();
+        //             }
 
-                    var valLabel: int := prevNode.omLabel + (labelGap / 2);
-                    var valNode: Node := new Node(valLabel, setVal, prevNode.index+1);
+        //             var valLabel: int := prevNode.omLabel + (labelGap / 2);
+        //             var valNode: Node := new Node(valLabel, setVal, prevNode.index+1);
 
-                    valNode.previous := prevNode;
-                    valNode.next := tail;
-                    prevNode.next := valNode;
-                    tail.previous := valNode;
-                }
+        //             valNode.previous := prevNode;
+        //             valNode.next := tail;
+        //             prevNode.next := valNode;
+        //             tail.previous := valNode;
+        //         }
 
-                omDsSeq := if setVal in omDsSeq then omDsSeq[..] else omDsSeq[..] + [setVal];
+        //         omDsSeq := if setVal in omDsSeq then omDsSeq[..] else omDsSeq[..] + [setVal];
 
-                iValSet := iValSet - { setVal };
-            }
-        }
+        //         iValSet := iValSet - { setVal };
+        //     }
+        // }
 
-        method prepend(valSet: set<int>)
-            // Check x doesn't exist in DS
-            requires exists val :: val in valSet && val !in omDsSeq
-            requires oldOmDsSeq == omDsSeq
-            // Check each value is unique
-            requires exists fstSeq, scndSeq, val :: omDsSeq == fstSeq + [val] + scndSeq && val !in fstSeq + scndSeq
-            // Check x is at the start of the DS always
-            ensures exists fstSeq, scndSeq, val :: omDsSeq == fstSeq + scndSeq && oldOmDsSeq == scndSeq && val in fstSeq && val in valSet
-            // Check each value is unique
-            ensures exists fstSeq, scndSeq, val :: omDsSeq == fstSeq + [val] + scndSeq && val !in fstSeq + scndSeq
-        {
-            var iValSet := valSet;
-            while ( iValSet != {} )
-                decreases iValSet;
-                modifies head.next
-            {
-                var setVal :| setVal in iValSet;
+        // method prepend(valSet: set<int>)
+        //     // Check x doesn't exist in DS
+        //     requires exists val :: val in valSet && val !in omDsSeq
+        //     requires oldOmDsSeq == omDsSeq
+        //     // Check each value is unique
+        //     requires exists fstSeq, scndSeq, val :: omDsSeq == fstSeq + [val] + scndSeq && val !in fstSeq + scndSeq
+        //     // Check x is at the start of the DS always
+        //     ensures exists fstSeq, scndSeq, val :: omDsSeq == fstSeq + scndSeq && oldOmDsSeq == scndSeq && val in fstSeq && val in valSet
+        //     // Check each value is unique
+        //     ensures exists fstSeq, scndSeq, val :: omDsSeq == fstSeq + [val] + scndSeq && val !in fstSeq + scndSeq
+        // {
+        //     var iValSet := valSet;
+        //     while ( iValSet != {} )
+        //         decreases iValSet;
+        //         modifies head.next
+        //     {
+        //         var setVal :| setVal in iValSet;
                 
-                // head.next is tail node in the worst case and never be null
-                // check whether existing element or not otherwise ignore to keep the uniqueness
-                var existSetVal: bool := element(setVal);
-                if(head.next != null && !existSetVal) {
-                    var nextNode: Node := head.next;
-                    var labelGap: int := nextNode.omLabel - head.omLabel;
+        //         // head.next is tail node in the worst case and never be null
+        //         // check whether existing element or not otherwise ignore to keep the uniqueness
+        //         var existSetVal: bool := element(setVal);
+        //         if(head.next != null && !existSetVal) {
+        //             var nextNode: Node := head.next;
+        //             var labelGap: int := nextNode.omLabel - head.omLabel;
 
-                    if(labelGap == 0) {
-                        relabel();
-                    }
+        //             if(labelGap == 0) {
+        //                 relabel();
+        //             }
 
-                    var valLabel: int := head.omLabel + (labelGap / 2);
-                    var valNode: Node := new Node(valLabel, setVal, nextNode.index-1);
+        //             var valLabel: int := head.omLabel + (labelGap / 2);
+        //             var valNode: Node := new Node(valLabel, setVal, nextNode.index-1);
 
-                    valNode.previous := head;
-                    valNode.next := nextNode;
-                    nextNode.previous := valNode;
-                    head.next := valNode;
-                }
+        //             valNode.previous := head;
+        //             valNode.next := nextNode;
+        //             nextNode.previous := valNode;
+        //             head.next := valNode;
+        //         }
 
-                omDsSeq := if setVal in omDsSeq then omDsSeq[..] else [setVal] + omDsSeq[..];
+        //         omDsSeq := if setVal in omDsSeq then omDsSeq[..] else [setVal] + omDsSeq[..];
 
-                iValSet := iValSet - { setVal };
-            }
-        }
+        //         iValSet := iValSet - { setVal };
+        //     }
+        // }
 
-        method remove(xNode: Node)
-            // Check x exists in DS
-            requires xNode.omValue in omDsSeq
-            // Check each value is unique
-            requires exists fstSeq, scndSeq, val :: omDsSeq == fstSeq + [val] + scndSeq && val !in fstSeq + scndSeq
-            // Check x doesn't exist in DS
-            ensures xNode.omValue !in omDsSeq
-        {
-            // xNode.next is tail node in the worst case and never be null
-            // xNode.previous is head node in the worst case and never be null
-            if(xNode.next != null && xNode.previous != null) {
-                var nextNode: Node := xNode.next;
-                var prevNode: Node := xNode.previous;
+        // method remove(xNode: Node)
+        //     // Check x exists in DS
+        //     requires xNode.omValue in omDsSeq
+        //     // Check each value is unique
+        //     requires exists fstSeq, scndSeq, val :: omDsSeq == fstSeq + [val] + scndSeq && val !in fstSeq + scndSeq
+        //     // Check x doesn't exist in DS
+        //     ensures xNode.omValue !in omDsSeq
+        // {
+        //     // xNode.next is tail node in the worst case and never be null
+        //     // xNode.previous is head node in the worst case and never be null
+        //     if(xNode.next != null && xNode.previous != null) {
+        //         var nextNode: Node := xNode.next;
+        //         var prevNode: Node := xNode.previous;
 
-                nextNode.previous := prevNode;
-                prevNode.next := nextNode;
+        //         nextNode.previous := prevNode;
+        //         prevNode.next := nextNode;
                 
-                reIndex();
-            }
+        //         reIndex();
+        //     }
 
-            omDsSeq := omDsSeq[..xNode.index] + omDsSeq[xNode.index+1..];
-        }
+        //     omDsSeq := omDsSeq[..xNode.index] + omDsSeq[xNode.index+1..];
+        // }
 
         method getXNode(x: int) returns (node: Node)
             // Check x exists in DS
@@ -421,8 +419,7 @@ module Collections {
         {
             var iNode: Node := head.next;
             while(iNode != tail)
-                invariant iNode == tail || iNode != tail
-                decreases iNode
+                decreases getLength() - getCurrentLength(iNode)
             {
                 if(iNode.omValue == x) {
                     node := iNode;
